

## Numerical Linear Algebra:

### Solvability of Linear Systems:

The shape of the matrix  $A$  bears considerable information about the solvability of  $Ax = b$ .

- First let us consider the case when the matrix  $A$  is wide, i.e.,  $n > m$ . Each column in a vector in  $\mathbb{R}^m$ . Since  $n > m$ , the  $n$  columns of  $A$  must be linearly dependent which implies that there exist some weights  $x_0 \neq 0$  which satisfies  $Ax_0 = 0$ . If we can solve  $Ax = b$  for some  $x$  then  $Ax(x + \alpha x_0) = Ax + \alpha Ax_0 = b + 0 = b$  for any  $\alpha \in \mathbb{R}$ . In summary, no wide system admits a unique solution.

Example:

Let's say:

$$A = \begin{bmatrix} 1 & 2 & 3 \\ 4 & 5 & 6 \end{bmatrix} \quad (2 \text{ rows} \times 3 \text{ columns})$$

This is a  $2 \times 3$  matrix  $\rightarrow$  wide matrix because 3 unknowns and only 2 equations.

Let's say:

$$\vec{b} = \begin{bmatrix} 14 \\ 32 \end{bmatrix}$$

We want to solve:

$$A\vec{x} = \vec{b} \Rightarrow \begin{bmatrix} 1 & 2 & 3 \\ 4 & 5 & 6 \end{bmatrix} \begin{bmatrix} x_1 \\ x_2 \\ x_3 \end{bmatrix} = \begin{bmatrix} 14 \\ 32 \end{bmatrix}$$

This gives two equations:

$$\begin{aligned} x_1 + 2x_2 + 3x_3 &= 14 \\ 4x_1 + 5x_2 + 6x_3 &= 32 \end{aligned}$$

There are infinitely many  $x_1, x_2, x_3$  that satisfy these two equations — because we have more unknowns than equations.

Non-unique solutions:

Because  $A$  has linearly dependent columns (we can express one column as a combination of others), there exists a non-zero vector  $\vec{x}_0$  such that:

$$A\vec{x}_0 = 0 \quad (\text{This is called the "null space" of } A)$$

Then, if we find one solution  $\vec{x}$  such that  $A\vec{x} = \vec{b}$ , then we can generate infinitely many other solutions by:

$$\vec{x}_{\text{new}} = \vec{x} + \alpha \vec{x}_0 \quad \text{for any } \alpha \in \mathbb{R}$$

Because:

$$A(\vec{x} + \alpha \vec{x}_0) = A\vec{x} + \alpha A\vec{x}_0 = \vec{b} + \alpha \cdot 0 = \vec{b}$$

- A **wide matrix** (more unknowns than equations) always has a **non-trivial null space** → meaning there are infinite solutions to  $A\vec{x} = \vec{b}$  if one exists.
- So: **You cannot have a unique solution.**
- Either:
  - No solution (if  $\vec{b} \notin \text{col}(A)$ ), or
  - **Infinitely many solutions**
- When  $A$  is tall, i.e.,  $m > n$ , then its  $n$  columns cannot possibly span the larger dimensional  $\mathbb{R}^m$ . For this reason, there could be some  $b_0 \notin \text{col } A$  so by definition  $Ax = b_0$  cannot be solved exactly for any  $x$ . In summary, for every tall matrix  $A$ , there exists a  $b_0$  such that  $Ax = b_0$  is not solvable.

Example:

Let:

$$\vec{b} = \begin{bmatrix} 5 \\ 11 \\ 17 \end{bmatrix}$$

We try to solve:

$$A\vec{x} = \vec{b} \Rightarrow \begin{bmatrix} 1 & 2 \\ 3 & 4 \\ 5 & 6 \end{bmatrix} \begin{bmatrix} x_1 \\ x_2 \end{bmatrix} = \begin{bmatrix} 5 \\ 11 \\ 17 \end{bmatrix}$$

This gives the system:

$$x_1 + 2x_2 = 5$$

$$3x_1 + 4x_2 = 11$$

$$5x_1 + 6x_2 = 17$$

If you try solving this, you'll find that **no single pair**  $(x_1, x_2)$  satisfies **all three** equations.

So, **no solution exists** → the system is **inconsistent**.

- A **tall matrix** has **more equations than unknowns**.
- Its columns cannot fill the whole space  $\mathbb{R}^m$ , only a smaller piece of it (the column space).
- So some target vectors  $\vec{b}_0$  are simply **out of reach**, and no matter what  $\vec{x}$  you try,  $A\vec{x}$  will never hit  $\vec{b}_0$ .
- $\oplus$  More equations than unknowns often means the system is **over-constrained** and may **not be solvable**.

## Gauss Elimination:

**Gaussian Elimination** (also called **row reduction**) is a method to solve a system of linear equations by transforming the system's **augmented matrix** into an **upper triangular form**, and then solving it using **back-substitution**.

- The method consists of two steps:
  - Forward Elimination:** the system is reduced to **upper triangular form**. A sequence of **elementary operations** is used.
  - Backward Substitution:** Solve the system starting from the last variable.

$$\begin{bmatrix} a_{11} & a_{12} & a_{13} \\ a_{21} & a_{22} & a_{23} \\ a_{31} & a_{32} & a_{33} \end{bmatrix} \begin{bmatrix} x_1 \\ x_2 \\ x_3 \end{bmatrix} = \begin{bmatrix} b_1 \\ b_2 \\ b_3 \end{bmatrix} \Rightarrow \begin{bmatrix} a_{11} & a_{12} & a_{13} \\ 0 & a_{22}' & a_{23}' \\ 0 & 0 & a_{33}' \end{bmatrix} \begin{bmatrix} x_1 \\ x_2 \\ x_3 \end{bmatrix} = \begin{bmatrix} b_1 \\ b_2' \\ b_3' \end{bmatrix}$$

### Example 1

Solve using Naive Gaussian Elimination:

Part1: Forward Elimination Step1: Eliminate  $x_1$  from equations 2, 3

$$x_1 + 2x_2 + 3x_3 = 8 \quad eq1 \text{ unchanged (pivot equation)}$$

$$2x_1 + 3x_2 + 2x_3 = 10 \quad eq2 \leftarrow eq2 - \left(\frac{2}{1}\right)eq1$$

$$3x_1 + x_2 + 2x_3 = 7 \quad eq3 \leftarrow eq3 - \left(\frac{3}{1}\right)eq1$$

$$\begin{aligned} x_1 + 2x_2 + 3x_3 &= 8 \\ -x_2 - 4x_3 &= -6 \\ -5x_2 - 7x_3 &= -17 \end{aligned}$$

Part1: Forward Elimination Step2: Eliminate  $x_2$  from equation 3

$$\begin{aligned} x_1 + 2x_2 + 3x_3 &= 8 & eq1 \text{ unchanged} \\ -x_2 - 4x_3 &= -6 & eq2 \text{ unchanged (pivot equation)} \end{aligned}$$

$$-5x_2 - 7x_3 = -17 \quad eq3 \leftarrow eq3 - \left(\frac{-5}{-1}\right)eq2$$

$$\Rightarrow \begin{cases} x_1 + 2x_2 + 3x_3 = 8 \\ -x_2 - 4x_3 = -6 \\ 13x_3 = 13 \end{cases}$$

## Backward Substitution

$$x_3 = \frac{b_3}{a_{3,3}} = \frac{13}{13} = 1$$

$$x_2 = \frac{b_2 - a_{2,3}x_3}{a_{2,2}} = \frac{-6 + 4x_3}{-1} = 2$$

$$x_1 = \frac{b_1 - a_{1,2}x_2 - a_{1,3}x_3}{a_{1,1}} = \frac{8 - 2x_2 - 3x_3}{a_{1,1}} = 1$$

The solution is  $\begin{bmatrix} x_1 \\ x_2 \\ x_3 \end{bmatrix} = \begin{bmatrix} 1 \\ 2 \\ 1 \end{bmatrix}$

## Example 2:

### Forward Elimination

$$\begin{bmatrix} 6 & -2 & 2 & 4 \\ 12 & -8 & 6 & 10 \\ 3 & -13 & 9 & 3 \\ -6 & 4 & 1 & -18 \end{bmatrix} \begin{bmatrix} x_1 \\ x_2 \\ x_3 \\ x_4 \end{bmatrix} = \begin{bmatrix} 16 \\ 26 \\ -19 \\ -34 \end{bmatrix}$$

#### Part 1 : Forward Elimination

Step1: Eliminate  $x_1$  from equations 2, 3, 4

$$\begin{bmatrix} 6 & -2 & 2 & 4 \\ 0 & -4 & 2 & 2 \\ 0 & -12 & 8 & 1 \\ 0 & 2 & 3 & -14 \end{bmatrix} \begin{bmatrix} x_1 \\ x_2 \\ x_3 \\ x_4 \end{bmatrix} = \begin{bmatrix} 16 \\ -6 \\ -27 \\ -18 \end{bmatrix}$$

Step2: Eliminate  $x_2$  from equations 3, 4

$$\begin{bmatrix} 6 & -2 & 2 & 4 \\ 0 & -4 & 2 & 2 \\ 0 & 0 & 2 & -5 \\ 0 & 0 & 4 & -13 \end{bmatrix} \begin{bmatrix} x_1 \\ x_2 \\ x_3 \\ x_4 \end{bmatrix} = \begin{bmatrix} 16 \\ -6 \\ -9 \\ -21 \end{bmatrix}$$

Step3: Eliminate  $x_3$  from equation 4

$$\begin{bmatrix} 6 & -2 & 2 & 4 \\ 0 & -4 & 2 & 2 \\ 0 & 0 & 2 & -5 \\ 0 & 0 & 0 & -3 \end{bmatrix} \begin{bmatrix} x_1 \\ x_2 \\ x_3 \\ x_4 \end{bmatrix} = \begin{bmatrix} 16 \\ -6 \\ -9 \\ -3 \end{bmatrix}$$

### Summary of the Forward Elimination :

$$\begin{bmatrix} 6 & -2 & 2 & 4 \\ 12 & -8 & 6 & 10 \\ 3 & -13 & 9 & 3 \\ -6 & 4 & 1 & -18 \end{bmatrix} \begin{bmatrix} x_1 \\ x_2 \\ x_3 \\ x_4 \end{bmatrix} = \begin{bmatrix} 16 \\ 26 \\ -19 \\ -34 \end{bmatrix} \Rightarrow \begin{bmatrix} 6 & -2 & 2 & 4 \\ 0 & -4 & 2 & 2 \\ 0 & 0 & 2 & -5 \\ 0 & 0 & 0 & -3 \end{bmatrix} \begin{bmatrix} x_1 \\ x_2 \\ x_3 \\ x_4 \end{bmatrix} = \begin{bmatrix} 16 \\ -6 \\ -9 \\ -3 \end{bmatrix}$$

$$\begin{bmatrix} 6 & -2 & 2 & 4 \\ 0 & -4 & 2 & 2 \\ 0 & 0 & 2 & -5 \\ 0 & 0 & 0 & -3 \end{bmatrix} \begin{bmatrix} x_1 \\ x_2 \\ x_3 \\ x_4 \end{bmatrix} = \begin{bmatrix} 16 \\ -6 \\ -9 \\ -3 \end{bmatrix}$$

Solve for  $x_4$ , then solve for  $x_3$ ,...solve for  $x_1$

$$x_4 = \frac{-3}{-3} = 1, \quad x_3 = \frac{-9+5}{2} = -2$$

$$x_2 = \frac{-6-2(-2)-2(1)}{-4} = 1, \quad x_1 = \frac{16+2(1)-2(-2)-4(1)}{6} = 3$$

$$\begin{array}{l} \text{To eliminate } x_1 \\ \left. \begin{array}{l} a_{ij} \leftarrow a_{ij} - \left( \frac{a_{i1}}{a_{11}} \right) a_{1j} \quad (1 \leq j \leq n) \\ b_i \leftarrow b_i - \left( \frac{a_{i1}}{a_{11}} \right) b_1 \end{array} \right\} 2 \leq i \leq n \end{array}$$

$$\begin{array}{l} \text{To eliminate } x_2 \\ \left. \begin{array}{l} a_{ij} \leftarrow a_{ij} - \left( \frac{a_{i2}}{a_{22}} \right) a_{2j} \quad (2 \leq j \leq n) \\ b_i \leftarrow b_i - \left( \frac{a_{i2}}{a_{22}} \right) b_2 \end{array} \right\} 3 \leq i \leq n \end{array}$$

$$\begin{array}{l} \text{To eliminate } x_k \\ \left. \begin{array}{l} a_{ij} \leftarrow a_{ij} - \left( \frac{a_{ik}}{a_{kk}} \right) a_{kj} \quad (k \leq j \leq n) \\ b_i \leftarrow b_i - \left( \frac{a_{ik}}{a_{kk}} \right) b_k \end{array} \right\} k+1 \leq i \leq n \end{array}$$

Continue until  $x_{n-1}$  is eliminated.